src/core/DY.Core.Trace.Base.fst
@@ -1,0 +1,349 @@
+module DY.Core.Trace.Base
+
+open DY.Core.Trace.Type
+open DY.Core.Bytes.Type
+open DY.Core.Label.Type
+
+/// Shorthands for trace and trace events.
+
+type trace_event = trace_event_ label
+type trace = trace_ label
+
+/// The length of a trace.
+
+val length: #label_t:Type -> trace_ label_t -> nat
+let rec length tr =
+  match tr with
+  | Nil -> 0
+  | Snoc init last -> length init + 1
+
+/// a type macro for timestamps (indices on the trace)
+
+type timestamp = nat
+
+(*** Prefix and trace_ extension ***)
+
+/// Compute the prefix of a trace.
+
+[@@ "opaque_to_smt"]
+val prefix: #label_t:Type -> tr:trace_ label_t -> i:timestamp{i <= length tr} -> trace_ label_t
+let rec prefix tr i =
+  if length tr = i then
+    tr
+  else
+    let Snoc tr_init _ = tr in
+    prefix tr_init i
+
+/// Express whether a trace is the extension of another.
+/// This is a crucial relation between traces,
+/// because the trace only grows during a protocol execution.
+
+[@@ "opaque_to_smt"]
+val grows: #label_t:Type -> trace_ label_t -> trace_ label_t -> prop
+let grows tr1 tr2 =
+  length tr1 <= length tr2 /\
+  tr1 == prefix tr2 (length tr1)
+
+/// It is used a lot in DY*, therefore we define an operator shorthand.
+
+let (<$) = grows
+
+val grows_induction_principle:
+  #label_t:Type ->
+  p:(trace_ label_t -> prop) ->
+  (tr:trace_ label_t -> ev:trace_event_ label_t -> Lemma (requires p tr) (ensures p (Snoc tr ev))) ->
+  tr1:trace_ label_t -> tr2:trace_ label_t ->
+  Lemma
+  (requires
+    p tr1 /\
+    tr1 <$ tr2
+  )
+  (ensures p tr2)
+let rec grows_induction_principle #label_t p pf tr1 tr2 =
+  reveal_opaque (`%grows) (grows #label_t);
+  norm_spec [zeta; delta_only [`%prefix]] (prefix #label_t);
+  if length tr1 = length tr2 then ()
+  else (
+    let Snoc init2 last2 = tr2 in
+    grows_induction_principle p pf tr1 init2;
+    pf init2 last2
+  )
+
+/// The relation <$ is reflexive.
+
+val grows_reflexive:
+  tr:trace ->
+  Lemma (tr <$ tr)
+  [SMTPat (tr <$ tr)]
+let grows_reflexive tr =
+  reveal_opaque (`%grows) (grows #label);
+  norm_spec [zeta; delta_only [`%prefix]] (prefix #label)
+
+/// The relation <$ is transitive.
+
+val grows_transitive:
+  tr1:trace -> tr2:trace -> tr3:trace ->
+  Lemma
+  (requires tr1 <$ tr2 /\ tr2 <$ tr3)
+  (ensures tr1 <$ tr3)
+  [SMTPat (tr1 <$ tr2); SMTPat (tr1 <$ tr3)]
+let rec grows_transitive tr1 tr2 tr3 =
+  reveal_opaque (`%grows) (grows #label);
+  norm_spec [zeta; delta_only [`%prefix]] (prefix #label);
+  if length tr2 >= length tr3 then
+    ()
+  else (
+    let Snoc tr3_init _ = tr3 in
+    grows_transitive tr1 tr2 tr3_init
+  )
+
+/// The prefix function outputs traces of the correct length.
+
+val length_prefix:
+  tr:trace -> i:timestamp{i <= length tr} ->
+  Lemma
+  (ensures length (prefix tr i) == i)
+  [SMTPat (length (prefix tr i))]
+let rec length_prefix tr i =
+  norm_spec [zeta; delta_only [`%prefix]] (prefix #label);
+  if length tr = i then ()
+  else
+    let Snoc tr_init _ = tr in
+    length_prefix tr_init i
+
+/// A trace which is the prefix of another is shorter.
+
+val length_grows:
+  tr1:trace -> tr2:trace ->
+  Lemma
+  (requires tr1 <$ tr2)
+  (ensures length tr1 <= length tr2)
+  [SMTPat (tr1 <$ tr2)]
+let length_grows tr1 tr2 =
+  reveal_opaque (`%grows) (grows #label)
+
+/// The prefix function outputs traces that are prefixes of the input.
+
+val prefix_grows:
+  tr:trace -> i:timestamp{i <= length tr} ->
+  Lemma
+  (ensures (prefix tr i) <$ tr)
+  //TODO: is this SMTPat dangerous? Should we restrict it to the "safe" on below?
+  [SMTPat (prefix tr i)]
+  //[SMTPat ((prefix tr i) <$ tr)]
+let prefix_grows tr i =
+  reveal_opaque (`%grows) (grows #label);
+  norm_spec [zeta; delta_only [`%prefix]] (prefix #label)
+
+val prefix_prefix_grows:
+  tr1:trace -> tr2:trace -> i1:timestamp -> i2:timestamp ->
+  Lemma
+  (requires
+    tr1 <$ tr2 /\
+    i1 <= length tr1 /\
+    i2 <= length tr2 /\
+    i1 <= i2
+  )
+  (ensures prefix tr1 i1 <$ prefix tr2 i2)
+  [SMTPat (prefix tr1 i1 <$ prefix tr2 i2)]
+  // Alternative SMT pattern if the above one doesn't trigger enough
+  // [SMTPat (prefix tr1 i1);
+  //  SMTPat (prefix tr2 i2);
+  //  SMTPat (tr1 <$ tr2)]
+let rec prefix_prefix_grows tr1 tr2 i1 i2 =
+  reveal_opaque (`%grows) (grows #label);
+  norm_spec [zeta; delta_only [`%prefix]] (prefix #label);
+  if i2 = length tr2 then ()
+  else if length tr1 = length tr2 then (
+    let Snoc tr1_init _ = tr1 in
+    let Snoc tr2_init _ = tr2 in
+    prefix_prefix_grows tr1_init tr2_init i1 i2
+  ) else (
+    let Snoc tr2_init _ = tr2 in
+    prefix_prefix_grows tr1 tr2_init i1 i2
+  )
+
+val prefix_prefix_eq:
+  tr1:trace -> tr2:trace -> i:timestamp ->
+  Lemma
+  (requires
+    tr1 <$ tr2 /\
+    i <= length tr1
+  )
+  (ensures prefix tr1 i == prefix tr2 i)
+  [SMTPat (prefix tr1 i);
+   SMTPat (prefix tr2 i);
+   SMTPat (tr1 <$ tr2)]
+let rec prefix_prefix_eq tr1 tr2 i =
+  reveal_opaque (`%grows) (grows #label);
+  norm_spec [zeta; delta_only [`%prefix]] (prefix #label);
+  if length tr1 = length tr2 then ()
+  else (
+    let Snoc tr2_init _ = tr2 in
+    prefix_prefix_eq tr1 tr2_init i
+  )
+
+(*** Event in the trace predicates ***)
+
+/// Retrieve the event at some timestamp in the trace.
+
+val get_event_at:
+  #label_t:Type ->
+  tr:trace_ label_t -> i:timestamp{i < length tr} ->
+  trace_event_ label_t
+let rec get_event_at tr i =
+  if i+1 = length tr then
+    let Snoc _ last = tr in
+    last
+  else (
+    let Snoc tr_init _ = tr in
+    get_event_at tr_init i
+  )
+
+/// Has some particular event been triggered at a some particular timestamp in the trace?
+
+val event_at:
+  #label_t:Type ->
+  trace_ label_t -> timestamp -> trace_event_ label_t ->
+  prop
+let event_at tr i e =
+  if i >= length tr then
+    False
+  else
+    e == get_event_at tr i
+
+/// Has some particular event been triggered in the trace (at any timestamp)?
+
+val event_exists:
+  #label_t:Type ->
+  trace_ label_t -> trace_event_ label_t ->
+  prop
+let event_exists tr e =
+  exists i. event_at tr i e
+
+/// An event in the trace stays here when the trace grows.
+
+val event_at_grows:
+  #label_t:Type ->
+  tr1:trace_ label_t -> tr2:trace_ label_t ->
+  i:timestamp -> e:trace_event_ label_t ->
+  Lemma
+  (requires event_at tr1 i e /\ tr1 <$ tr2)
+  (ensures event_at tr2 i e)
+  [SMTPat (event_at tr1 i e); SMTPat (tr1 <$ tr2)]
+let rec event_at_grows #label_t tr1 tr2 i e =
+  reveal_opaque (`%grows) (grows #label_t);
+  norm_spec [zeta; delta_only [`%prefix]] (prefix #label_t);
+  if i >= length tr1 then ()
+  else if length tr1 >= length tr2 then ()
+  else (
+    let Snoc tr2_init _ = tr2 in
+    event_at_grows tr1 tr2_init i e
+  )
+
+/// Shorthand predicates.
+
+/// Has a message been sent on the network?
+
+val msg_sent_on_network: trace -> bytes -> prop
+let msg_sent_on_network tr msg =
+  event_exists tr (MsgSent msg)
+
+/// Has some state been stored by a principal?
+
+val state_was_set: trace -> principal -> state_id -> bytes -> prop
+let state_was_set tr prin sess_id content =
+  event_exists tr (SetState prin sess_id content)
+
+/// Has a principal been corrupt?
+
+val was_corrupt: #label_t:Type -> trace_ label_t -> principal -> state_id -> prop
+let was_corrupt tr prin sess_id =
+  event_exists tr (Corrupt prin sess_id)
+
+/// Has a (custom, protocol-specific) event been triggered at some timestamp?
+
+val event_triggered_at: trace -> timestamp -> principal -> string -> bytes -> prop
+let event_triggered_at tr i prin tag content =
+  event_at tr i (Event prin tag content)
+
+/// Has a (custom, protocol-specific) event been triggered (at any timestamp)?
+
+val event_triggered: trace -> principal -> string -> bytes -> prop
+let event_triggered tr prin tag content =
+  exists i. event_triggered_at tr i prin tag content
+
+/// An event being triggered at some time stays triggered as the trace grows.
+
+val event_triggered_grows:
+  tr1:trace -> tr2:trace ->
+  prin:principal -> tag:string -> content:bytes  ->
+  Lemma
+  (requires event_triggered tr1 prin tag content /\ tr1 <$ tr2)
+  (ensures event_triggered tr2 prin tag content)
+  [SMTPat (event_triggered tr1 prin tag content); SMTPat (tr1 <$ tr2)]
+let event_triggered_grows tr1 tr2 prin tag content = ()
+
+/// Has a random bytestring been generated at some timestamp?
+
+val rand_generated_at: trace -> timestamp -> bytes -> prop
+let rand_generated_at tr i b =
+  match b with
+  | Rand usg len time ->
+    time == i /\ (exists lab. event_at tr i (RandGen usg lab len))
+  | _ -> False
+
+(*** Forgetting labels ***)
+
+/// Functions to replace labels in a trace by `()`.
+/// This is useful to use labels that are predicates on `trace_ unit`
+/// with actual traces that are `trace_ label`.
+/// See `DY.Core.Label.Type` for more information
+
+val trace_event_forget_labels:
+  trace_event ->
+  trace_event_ unit
+let trace_event_forget_labels ev =
+  match ev with
+  | MsgSent msg -> MsgSent msg
+  | RandGen usg lab len -> RandGen usg () len
+  | Corrupt prin sess_id -> Corrupt prin sess_id
+  | SetState prin sess_id content -> SetState prin sess_id content
+  | Event prin tag content -> Event prin tag content
+
+val trace_forget_labels:
+  trace ->
+  trace_ unit
+let rec trace_forget_labels tr =
+  match tr with
+  | Nil -> Nil
+  | Snoc init last ->
+    Snoc (trace_forget_labels init) (trace_event_forget_labels last)
+
+val length_trace_forget_labels:
+  tr:trace ->
+  Lemma (length (trace_forget_labels tr) == length tr)
+let rec length_trace_forget_labels tr =
+  match tr with
+  | Nil -> ()
+  | Snoc init last -> length_trace_forget_labels init
+
+val trace_forget_labels_later:
+  tr1:trace -> tr2:trace ->
+  Lemma
+  (requires tr1 <$ tr2)
+  (ensures (trace_forget_labels tr1) <$ (trace_forget_labels tr2))
+let rec trace_forget_labels_later tr1 tr2 =
+  reveal_opaque (`%grows) (grows #unit);
+  norm_spec [zeta; delta_only [`%prefix]] (prefix #unit);
+  reveal_opaque (`%grows) (grows #label);
+  norm_spec [zeta; delta_only [`%prefix]] (prefix #label);
+  if length tr1 = length tr2 then (
+    match tr1, tr2 with
+    | Nil, Nil -> ()
+    | Snoc tr1_init _, Snoc tr2_init _ -> ()
+  ) else (
+    let Snoc tr2_init tr2_last = tr2 in
+    trace_forget_labels_later tr1 tr2_init
+  )
+
